ulib/FStar.Integers.fst
@@ -2,17 +2,344 @@ module FStar.Integers
 
 #set-options "--initial_ifuel 1 --max_ifuel 1 --initial_fuel 0 --max_fuel 0"
 
-let within_bounds (x:int) : prop = admit ()
+type signedness =
+  | Signed
+  | Unsigned
 
-let v (x:int)
-  : Tot (y:int{(within_bounds y)})
-  = admit ()
+type width =
+  | W8
+  | W16
+  | W31
+  | W32
+  | W63
+  | W64
+  | W128
+  | Winfinite
 
-let foo (x:int) (y:int)
-  : Tot (z:int{normalize (eq2 #int (v z) (v x + v y))})
-  = admit ()
-  
-let bar (x:int)
-  : Tot (z:int{v z == foo (v x) (v x)})
-  = admit ()
+let fixed_width = w:width{w <> Winfinite}
 
+let nat_of_width = function
+  | W8   -> Some 8
+  | W16  -> Some 16
+  | W31  -> Some 31
+  | W32  -> Some 32
+  | W63  -> Some 63
+  | W64  -> Some 64
+  | W128 -> Some 128
+  | Winfinite -> None
+
+let nat_of_fixed_width (w:fixed_width) =
+  match nat_of_width w with
+  | Some v -> v
+
+let int_t (s:signedness) (w:width) : Tot Type0 =
+  match s, w with
+  | Unsigned, Winfinite -> nat
+  | Unsigned, W8 -> FStar.UInt8.t
+  | Unsigned, W16 -> FStar.UInt16.t
+  | Unsigned, W31 -> FStar.UInt31.t
+  | Unsigned, W32 -> FStar.UInt32.t
+  | Unsigned, W63 -> FStar.UInt63.t
+  | Unsigned, W64 -> FStar.UInt64.t
+  | Unsigned, W128 -> FStar.UInt128.t
+  | Signed, Winfinite -> int
+  | Signed, W8 -> FStar.Int8.t
+  | Signed, W16 -> FStar.Int16.t
+  | Signed, W31 -> FStar.Int31.t
+  | Signed, W32 -> FStar.Int32.t
+  | Signed, W63 -> FStar.Int63.t
+  | Signed, W64 -> FStar.Int64.t
+  | Signed, W128 -> FStar.Int128.t
+
+abstract
+let nat_size (x:int) : prop =
+  x >= 0
+let reveal_nat_size x
+  : Lemma (nat_size x <==> x >= 0)
+          [SMTPat (nat_size x)]
+  = ()
+
+abstract
+let uint_size (x:int) (n:nat) : prop =
+    FStar.UInt.size x n
+let reveal_uint_size x n
+  : Lemma (uint_size x n <==> FStar.UInt.size x n)
+          [SMTPat (uint_size x n)]
+  = ()
+
+abstract
+let int_size (x:int) (n:pos) : prop =
+    FStar.Int.size x n
+let reveal_int_size x n
+  : Lemma (int_size x n <==> FStar.Int.size x n)
+          [SMTPat (int_size x n)]
+  = ()
+
+let within_bounds (s:signedness) (w:width) (x:int) : prop =
+  match s, nat_of_width w with
+  | Signed,   None   -> True
+  | Unsigned, None   -> nat_size x
+  | Signed  , Some n -> int_size x n
+  | Unsigned, Some n -> uint_size x n
+
+let v (#s:signedness) (#w:width) (x:int_t s w)
+  : Tot (y:int_t Signed Winfinite{normalize (within_bounds s w y)})
+  = match s with
+    | Unsigned ->
+      (match w with
+       | Winfinite -> (x <: nat)
+       | W8 -> FStar.UInt8.v x
+       | W16 -> FStar.UInt16.v x
+       | W31 -> FStar.UInt31.v x
+       | W32 -> FStar.UInt32.v x
+       | W63 -> FStar.UInt63.v x
+       | W64 -> FStar.UInt64.v x
+       | W128 -> FStar.UInt128.v x)
+    | Signed ->
+      (match w with
+       | Winfinite -> x
+       | W8 -> FStar.Int8.v x
+       | W16 -> FStar.Int16.v x
+       | W31 -> FStar.Int31.v x
+       | W32 -> FStar.Int32.v x
+       | W63 -> FStar.Int63.v x
+       | W64 -> FStar.Int64.v x
+       | W128 -> FStar.Int128.v x)
+
+let u   (#s:signedness) (#w:width)
+        (x:int_t Signed Winfinite{normalize (within_bounds s w x)})
+  : Tot (y:int_t s w{normalize (v x == v y)})
+  = match s with
+    | Unsigned ->
+      (match w with
+       | Winfinite -> (x <: nat)
+       | W8 -> FStar.UInt8.uint_to_t x
+       | W16 -> FStar.UInt16.uint_to_t x
+       | W31 -> FStar.UInt31.uint_to_t x
+       | W32 -> FStar.UInt32.uint_to_t x
+       | W63 -> FStar.UInt63.uint_to_t x
+       | W64 -> FStar.UInt64.uint_to_t x
+       | W128 -> FStar.UInt128.uint_to_t x)
+    | Signed ->
+      (match w with
+       | Winfinite -> x
+       | W8 -> FStar.Int8.int_to_t x
+       | W16 -> FStar.Int16.int_to_t x
+       | W31 -> FStar.Int31.int_to_t x
+       | W32 -> FStar.Int32.int_to_t x
+       | W63 -> FStar.Int63.int_to_t x
+       | W64 -> FStar.Int64.int_to_t x
+       | W128 -> FStar.Int128.int_to_t x)
+
+abstract let cast (#s:signedness) (#s':signedness)
+         (#w:width)      (#w':width)
+         (from:int_t s w{normalize (within_bounds s' w' (v from))})
+   : Tot (to:int_t s' w'{normalize (v from == v to)})
+   = u (v from)
+
+unfold
+let ( + ) (#s:signedness) (#w:width)
+          (x:int_t s w)
+          (y:int_t s w{normalize (within_bounds s w (v x + v y))})
+  : Tot   (z:int_t s w{normalize (v z = v x + v y)})
+  = match s, w with
+    | _, Winfinite -> x + y
+    | Unsigned, W8   -> FStar.UInt8.(x +^ y)
+    | Unsigned, W16  -> FStar.UInt16.(x +^ y)
+    | Unsigned, W31  -> FStar.UInt31.(x +^ y)
+    | Unsigned, W32  -> FStar.UInt32.(x +^ y)
+    | Unsigned, W63  -> FStar.UInt63.(x +^ y)
+    | Unsigned, W64  -> FStar.UInt64.(x +^ y)
+    | Unsigned, W128 -> FStar.UInt128.(x +^ y)
+    | Signed, W8   -> FStar.Int8.(x +^ y)
+    | Signed, W16  -> FStar.Int16.(x +^ y)
+    | Signed, W31  -> FStar.Int31.(x +^ y)
+    | Signed, W32  -> FStar.Int32.(x +^ y)
+    | Signed, W63  -> FStar.Int63.(x +^ y)
+    | Signed, W64  -> FStar.Int64.(x +^ y)
+    | Signed, W128 -> FStar.Int128.(x +^ y)
+
+unfold
+let ( +? ) (#w:width)
+           (x:int_t Unsigned w)
+           (y:int_t Unsigned w)
+  : Tot    (z:int_t Unsigned w{normalize (within_bounds Unsigned w (v x + v y) ==> v z = v x + v y)})
+  = match w with
+    | Winfinite -> x + y
+    | W8 -> FStar.UInt8.(x +?^ y)
+    | W16 -> FStar.UInt16.(x +?^ y)
+    | W31 -> FStar.UInt31.(x +?^ y)
+    | W32 -> FStar.UInt32.(x +?^ y)
+    | W63 -> FStar.UInt63.(x +?^ y)
+    | W64 -> FStar.UInt64.(x +?^ y)
+    | W128 -> FStar.UInt128.(x +?^ y)
+
+let modulo (s:signedness) (x:int) (y:pos{s=Signed ==> y%2=0}) =
+  match s with
+  | Unsigned ->  x % y
+  | _ -> FStar.Int.(x @% y)
+
+unfold
+let ( +% ) (#w:fixed_width)
+           (x:int_t Unsigned w)
+           (y:int_t Unsigned w)
+  : Tot    (z:int_t Unsigned w{v z == modulo Unsigned (v x + v y) (pow2 (nat_of_fixed_width w))})
+  = match w with
+    | W8 -> FStar.UInt8.(x +%^ y)
+    | W16 -> FStar.UInt16.(x +%^ y)
+    | W31 -> FStar.UInt31.(x +%^ y)
+    | W32 -> FStar.UInt32.(x +%^ y)
+    | W63 -> FStar.UInt63.(x +%^ y)
+    | W64 -> FStar.UInt64.(x +%^ y)
+    | W128 -> FStar.UInt128.(x +%^ y)
+
+unfold
+let op_Subtraction (#s:signedness) (#w:width)
+                   (x:int_t s w)
+                   (y:int_t s w{within_bounds s w (v x - v y)})
+    : Tot          (z:int_t s w{v z = v x - v y})
+  = match s, w with
+    | _, Winfinite -> x - y
+    | Unsigned, W8 -> FStar.UInt8.(x -^ y)
+    | Unsigned, W16 -> FStar.UInt16.(x -^ y)
+    | Unsigned, W31 -> FStar.UInt31.(x -^ y)
+    | Unsigned, W32 -> FStar.UInt32.(x -^ y)
+    | Unsigned, W63 -> FStar.UInt63.(x -^ y)
+    | Unsigned, W64 -> FStar.UInt64.(x -^ y)
+    | Unsigned, W128 -> FStar.UInt128.(x -^ y)
+    | Signed, W8 -> FStar.Int8.(x -^ y)
+    | Signed, W16 -> FStar.Int16.(x -^ y)
+    | Signed, W31 -> FStar.Int31.(x -^ y)
+    | Signed, W32 -> FStar.Int32.(x -^ y)
+    | Signed, W63 -> FStar.Int63.(x -^ y)
+    | Signed, W64 -> FStar.Int64.(x -^ y)
+    | Signed, W128 -> FStar.Int128.(x -^ y)
+
+unfold
+let op_Subtraction_Question
+        (#w:width)
+        (x:int_t Unsigned w)
+        (y:int_t Unsigned w)
+  : Tot (z:int_t Unsigned w{within_bounds Unsigned w (v x - v y) ==> v z = v x - v y})
+  = match w with
+    | Winfinite -> if v x - v y >= 0 then x - y else 0
+    | W8 -> FStar.UInt8.(x -?^ y)
+    | W16 -> FStar.UInt16.(x -?^ y)
+    | W31 -> FStar.UInt31.(x -?^ y)
+    | W32 -> FStar.UInt32.(x -?^ y)
+    | W63 -> FStar.UInt63.(x -?^ y)
+    | W64 -> FStar.UInt64.(x -?^ y)
+    | W128 -> FStar.UInt128.(x -?^ y)
+
+unfold
+let op_Subtraction_Percent
+         (#w:fixed_width)
+         (x:int_t Unsigned w)
+         (y:int_t Unsigned w)
+  : Tot  (z:int_t Unsigned w{v z = modulo Unsigned (v x - v y) (pow2 (nat_of_fixed_width w))})
+  = match w with
+    | W8 -> FStar.UInt8.(x -%^ y)
+    | W16 -> FStar.UInt16.(x -%^ y)
+    | W31 -> FStar.UInt31.(x -%^ y)
+    | W32 -> FStar.UInt32.(x -%^ y)
+    | W63 -> FStar.UInt63.(x -%^ y)
+    | W64 -> FStar.UInt64.(x -%^ y)
+    | W128 -> FStar.UInt128.(x -%^ y)
+
+open FStar.Mul
+
+unfold
+let ( * ) (#s:signedness) (#w:width{w <> W128})
+          (x:int_t s w)
+          (y:int_t s w{within_bounds s w (v x * v y)})
+  : Tot   (z:int_t s w{v z = v x * v y})
+  = match s, w with
+    | _, Winfinite -> x * y
+    | Unsigned, W8 -> FStar.UInt8.(x *^ y)
+    | Unsigned, W16 -> FStar.UInt16.(x *^ y)
+    | Unsigned, W31 -> FStar.UInt31.(x *^ y)
+    | Unsigned, W32 -> FStar.UInt32.(x *^ y)
+    | Unsigned, W63 -> FStar.UInt63.(x *^ y)
+    | Unsigned, W64 -> FStar.UInt64.(x *^ y)
+    | Signed, W8 -> FStar.Int8.(x *^ y)
+    | Signed, W16 -> FStar.Int16.(x *^ y)
+    | Signed, W31 -> FStar.Int31.(x *^ y)
+    | Signed, W32 -> FStar.Int32.(x *^ y)
+    | Signed, W63 -> FStar.Int63.(x *^ y)
+    | Signed, W64 -> FStar.Int64.(x *^ y)
+    | Signed, W128 -> FStar.Int128.(x *^ y)
+
+unfold
+let ( *? ) (#w:width{w <> W128})
+           (x:int_t Unsigned w)
+           (y:int_t Unsigned w)
+  : Tot    (z:int_t Unsigned w{within_bounds Unsigned w (v x * v y) ==> v z = v x * v y})
+  = match w with
+    | Winfinite -> x * y
+    | W8 -> FStar.UInt8.(x *?^ y)
+    | W16 -> FStar.UInt16.(x *?^ y)
+    | W31 -> FStar.UInt31.(x *?^ y)
+    | W32 -> FStar.UInt32.(x *?^ y)
+    | W63 -> FStar.UInt63.(x *?^ y)
+    | W64 -> FStar.UInt64.(x *?^ y)
+
+unfold
+let ( *% ) (#w:fixed_width{w <> W128})
+           (x:int_t Unsigned w)
+           (y:int_t Unsigned w)
+  : Tot    (z:int_t Unsigned w{v z = modulo Unsigned (v x * v y) (pow2 (nat_of_fixed_width w))})
+  = match w with
+    | W8 -> FStar.UInt8.(x *%^ y)
+    | W16 -> FStar.UInt16.(x *%^ y)
+    | W31 -> FStar.UInt31.(x *%^ y)
+    | W32 -> FStar.UInt32.(x *%^ y)
+    | W63 -> FStar.UInt63.(x *%^ y)
+    | W64 -> FStar.UInt64.(x *%^ y)
+
+unfold let nat        = int_t Unsigned Winfinite
+unfold let uint_8   = int_t Unsigned W8
+unfold let uint_16  = int_t Unsigned W16
+unfold let uint_31  = int_t Unsigned W31
+unfold let uint_32  = int_t Unsigned W32
+unfold let uint_63  = int_t Unsigned W63
+unfold let uint_64  = int_t Unsigned W64
+
+unfold let int       = int_t Signed Winfinite
+unfold let int_8   = int_t Signed W8
+unfold let int_16  = int_t Signed W16
+unfold let int_31  = int_t Signed W31
+unfold let int_32  = int_t Signed W32
+unfold let int_63  = int_t Signed W63
+unfold let int_64  = int_t Signed W64
+unfold let int_128 = int_t Signed W128
+
+unfold
+let ok (#s:signedness) (#w:width)
+       (op:(int_t Signed Winfinite
+          -> int_t Signed Winfinite
+          -> int_t Signed Winfinite))
+       (x:int_t s w)
+       (y:int_t s w)
+   = normalize (within_bounds s w (op (v x) (v y)))
+////////////////////////////////////////////////////////////////////////////////
+//Test
+////////////////////////////////////////////////////////////////////////////////
+let f_int (x:int) (y:int) = x + y
+let f_nat (x:nat) (y:nat) = x + y
+let f_uint_8 (x:uint_8) (y:uint_8{ok (+) x y}) = x + y
+let f_int_16 (x:int_16) (y:int_16{ok (+) x y}) = x + y
+let g (x:uint_32) (y:uint_32{ok ( * ) y y /\ ok (+) x (y * y)}) = x + y * y
+let h (x:Prims.nat) (y:Prims.nat): nat  = u x + u y
+(* TODO: A bit boring ... *)
+(* let op_Slash_Hat = div *)
+(* let op_Percent_Hat = rem *)
+(* let op_Hat_Hat = logxor *)
+(* let op_Amp_Hat = logand *)
+(* let op_Bar_Hat = logor *)
+(* let op_Less_Less_Hat = shift_left *)
+(* let op_Greater_Greater_Hat = shift_right *)
+(* let op_Equals_Hat = eq *)
+(* let op_Greater_Hat = gt *)
+(* let op_Greater_Equals_Hat = gte *)
+(* let op_Less_Hat = lt *)
+(* let op_Less_Equals_Hat = lte *)
